simple dao example

Coq/DAO.v
@@ -5,9 +5,389 @@ Require Import loo_reduction_properties.
 Require Import decoupled_classical_properties.
 Require Import decoupling.
 Require Import function_operations.
+Require Import hoare.
 Require Import List.
 Require Import CpdtTactics.
 Require Import Coq.Logic.FunctionalExtensionality.
+
+Module SimpleDAO.
+
+  Definition a := bnd 1.
+
+  Definition b := bnd 2.
+
+  Definition c := bnd 3.
+
+  Definition x := bnd 4.
+
+  Definition y := bnd 5.
+
+  Definition z := bnd 6.
+  
+  Definition id := bnd 7.
+
+  Definition amt := bnd 8.
+
+  Definition name := fieldID 1.
+
+  Definition balance := fieldID 2.
+
+  Definition ether := fieldID 3.
+
+  Definition send := methID 1.
+
+  Definition repay := methID 2.
+
+  Definition repayDef1 := (a ≔′ e_nat 0) ;;
+                          ((r_ x ≔ (this ◌ balance)) ;;
+                           ((r_ y ≔ (this ◌ ether)) ;;
+                            ((b ≔′ e_minus (e_var y) (e_var x)) ;;
+                             ((s_if ((e_var x) ⩽ (e_var y))
+                                    (
+                                      s_if (e_var id ⩵ e_acc_f (e_var this) name)
+                                           (this ◌ ether ≔ (r_ b) ;;
+                                            (s_meth z id send (update amt x empty) ;;
+                                             (this ◌ balance ≔ (r_ a))))
+                                           (s_rtrn a)
+                                    )
+                                    (s_rtrn a)) ;;
+                              s_rtrn a)))).
+
+  Definition repayDef2 := (a ≔′ e_nat 0) ;;
+                          ((r_ x ≔ (this ◌ balance)) ;;
+                           ((r_ y ≔ (this ◌ ether)) ;;
+                            ((b ≔′ e_minus (e_var y) (e_var x)) ;;
+                             ((s_if ((e_var x) ⩽ (e_var y))
+                                    (
+                                      s_if (e_var id ⩵ e_acc_f (e_var this) name)
+                                           (this ◌ ether ≔ (r_ b) ;;
+                                            ((this ◌ balance ≔ (r_ a)) ;;
+                                             s_meth z id send (update amt x empty)))
+                                           (s_rtrn a)
+                                    )
+                                    (s_rtrn a)) ;;
+                              s_rtrn a)))).
+
+  Definition DAO := classID 1.
+
+  Definition DAODef1 := clazz DAO
+                              (name :: balance :: ether :: nil)
+                              (update repay ((id :: nil),repayDef1) empty)
+                              empty.
+
+  Definition DAODef2 := clazz DAO
+                              (name :: balance :: ether :: nil)
+                              (update repay ((id :: nil),repayDef2) empty)
+                              empty.
+
+  Definition DAOModule1 := update DAO DAODef1 empty.
+
+  Definition DAOModule2 := update DAO DAODef2 empty.
+
+  Definition DAOSPEC1 :=
+    (∀x∙ ((a_class (a♢ 0) DAO ∧
+           (a_expr (ex_acc_f (e♢ 0) balance ⩽′ (ex_acc_f (e♢ 0) ether))))
+            ⟶
+            (a_next (a_expr (ex_acc_f (e♢ 0) balance ⩽′ (ex_acc_f (e♢ 0) ether))))
+    )).
+
+  Definition Client := classID 2.
+
+  Definition sendBody := s_rtrn amt.
+
+  Definition ClientDef := clazz Client
+                                nil
+                                (update send (amt :: nil, sendBody) empty)
+                                empty.
+
+  Definition ClientModule := update Client ClientDef empty.
+
+  Definition αthis := address 0.
+
+  Definition Object := new Object empty.
+
+  Definition χ0 := (update αthis Object empty).
+
+  Definition β0 := update this (v_addr αthis) empty.
+
+  Definition client := bnd 9.
+
+  Definition αclient := address 1.
+
+  Definition αDAO := address 2.
+
+  Definition clientObj := new Client empty.
+
+  Definition daoFields := update name (v_addr αclient)
+                                 (update balance (v_nat 10)
+                                         (update ether (v_nat 10)
+                                                 empty)).
+
+  Definition DAOObj := new DAO daoFields.
+
+  Definition dao := bnd 10.
+
+  Definition ten := bnd 11.
+
+  Definition daoParams := update name client
+                                 (update balance ten
+                                         (update ether ten
+                                                 empty)).
+
+  Definition s0 := (s_new client Client empty) ;;
+                   ((ten ≔′ (e_nat 10)) ;;
+                    ((s_new dao DAO daoParams) ;;
+                     (s_meth c dao repay (update id client empty) ;;
+                      (s_rtrn c)))).
+
+  Definition c0 := c_stmt s0.
+
+  Definition ϕ0 := frm β0 c0.
+
+  Definition σ0 := (χ0, ϕ0 :: nil).
+
+  Definition χA := (update αDAO DAOObj
+                           (update αclient clientObj χ0)).
+
+  Definition βA := (update dao (v_addr αDAO)
+                           (update ten (v_nat 10)
+                                   (update client (v_addr αclient) β0))).
+
+  Definition sA := (s_meth c dao repay (update id client empty) ;;
+                    s_rtrn c).
+
+  Definition cA := c_stmt sA.
+
+  Definition ϕA := frm βA cA.
+
+  Definition σA := (χA, ϕA :: nil).
+
+  Definition updatedDAO := new DAO
+                               (update ether (v_nat 0) daoFields).
+
+  Definition χB := update αDAO updatedDAO
+                          χA.
+
+  Definition βB' := update b (v_nat 0)
+                           (update y (v_nat 10)
+                                   (update x (v_nat 10)
+                                           (update a (v_nat 0)
+                                                   (update this (v_addr αDAO) empty)))).
+
+  Definition sB' := s_rtrn a.
+
+  Definition cB' := c_hole z sB'.
+
+  Definition ϕB' := frm βB' cB'.
+
+  Definition βB := (update this (v_addr αclient) empty).
+
+  Definition cB := c_stmt (s_rtrn a).
+
+  Definition ϕB := frm βB cB.
+
+  Definition σB := (χB, ϕB :: ϕB' :: nil).
+
+  Lemma exists_linking_of_DAOModule1_ClientModule :
+    exists M, DAOModule1 ⋄ ClientModule ≜ M.
+  Proof.
+
+  Admitted.
+
+  Lemma σ0_initial :
+    initial σ0.
+  Proof.
+
+  Admitted.
+
+  Lemma σ0_reduces_to_σA :
+    DAOModule1 ⦂ ClientModule ⦿ σ0 ⤳⋆ σA.
+  Proof.
+    
+  Admitted.
+
+  Lemma σA_maps_αDAO_to_DAOObj :
+    ⟦ αDAO ↦ DAOObj ⟧ ∈ σA.
+  Proof.
+    repeat map_rewrite;
+      simpl.
+    unfold χA.
+    repeat map_rewrite.
+  Qed.
+
+  Lemma σA_reduces_to_σB :
+    DAOModule1 ⦂ ClientModule ⦿ σA ⤳ σB.
+  Proof.
+
+  Admitted.
+
+  Lemma balance_neq_ether :
+    balance <> ether.
+  Proof.
+    unfold balance, ether;
+      crush.
+  Qed.
+
+  Lemma balance_neq_name :
+    balance <> name.
+  Proof.
+    unfold balance, name;
+      crush.
+  Qed.
+
+  Lemma σA_satisfies_SPEC_premise :
+    DAOModule1 ⦂ ClientModule ◎ σ0 … σA
+               ⊨ (a_class (a_ αDAO) DAO
+                  ∧ a_expr (ex_acc_f (e_ αDAO) balance ⩽′ ex_acc_f (e_ αDAO) ether)).
+  Proof.
+    a_prop.
+
+    - apply sat_class with (o:=DAOObj);
+        auto.
+
+    - destruct exists_linking_of_DAOModule1_ClientModule as [M].
+      apply sat_exp with (M:=M)(e':=e_acc_f (e_val (v_addr αDAO)) balance ⩽
+                                            e_acc_f (e_val (v_addr αDAO)) ether);
+        auto.
+      + apply decoupling.is_if;
+          auto with chainmail_db.
+      + apply v_if_false.
+        * apply v_nlt with (i1:=10)(i2:=10);
+            [| |crush].
+          ** apply v_f_heap with (α:=αDAO)(o:=DAOObj);
+               eauto with loo_db.
+          ** apply v_f_heap with (α:=αDAO)(o:=DAOObj);
+               eauto with loo_db.
+        * apply v_if_true;
+            auto with loo_db.
+          apply v_equals with (v:=v_nat 10).
+          ** apply v_f_heap with (α:=αDAO)(o:=DAOObj);
+               eauto with loo_db.
+          ** apply v_f_heap with (α:=αDAO)(o:=DAOObj);
+               eauto with loo_db.
+  Qed.
+
+  Lemma DAO1_nsat :
+    ~ DAOModule1 ⊨m DAOSPEC1.
+  Proof.
+    unfold mdl_sat.
+    intro Hcontra.
+    specialize (Hcontra ClientModule).
+    specialize (Hcontra σ0 σA exists_linking_of_DAOModule1_ClientModule).
+    specialize (Hcontra σ0_initial).
+    specialize (Hcontra σ0_reduces_to_σA).
+    inversion Hcontra;
+      subst;
+      simpl in *.
+    specialize (H4 αDAO DAOObj σA_maps_αDAO_to_DAOObj).
+    a_prop.
+    assert (DAOModule1 ⦂ ClientModule ◎ σ0 … σA
+                       ⊨ (a_class (a_ αDAO) DAO
+                          ∧ a_expr (ex_acc_f (e_ αDAO) balance ⩽′ ex_acc_f (e_ αDAO) ether)));
+      [apply σA_satisfies_SPEC_premise|auto_specialize].
+    repeat a_prop.
+    inversion H4;
+      subst.
+    unfold σA in H2;
+      repeat simpl_crush. 
+    assert (DAOModule1 ⦂ ClientModule ⦿ σA ⤳ σB);
+      [apply σA_reduces_to_σB|].
+    unique_reduction_auto.
+
+    inversion H9;
+      subst.
+    repeat match goal with
+           | [H : is_exp _ _ |- _] =>
+             inversion H;
+               subst;
+               clear H
+           end.
+    inversion H11;
+      subst.
+    - inversion H12;
+        subst.
+      
+      inversion H6;
+        subst.
+      inversion H7;
+        subst.
+      repeat map_rewrite.
+      simpl in H16.
+      unfold χB in H16.
+      repeat map_rewrite.
+      inversion H16;
+        subst.
+      simpl in *.
+      repeat map_rewrite.
+      assert (balance <> ether);
+        [apply balance_neq_ether|eq_auto].
+      unfold daoFields in *;
+        repeat map_rewrite.
+      assert (balance <> name);
+        [apply balance_neq_name|eq_auto; simpl_crush].
+
+      inversion H10;
+        subst.
+      inversion H17;
+        subst.
+      repeat map_rewrite;
+        simpl in *;
+        unfold χB in *;
+        repeat map_rewrite;
+        simpl_crush.
+      simpl in *;
+        repeat map_rewrite;
+        simpl_crush.
+      crush.
+
+    - inversion H13;
+        subst.
+
+      + inversion H14;
+          subst.
+        inversion H8;
+          subst.
+        repeat map_rewrite.
+        simpl in *.
+        unfold χB in *.
+        repeat map_rewrite.
+        inversion H6;
+          subst.
+        simpl in *.
+        simpl_crush.
+        simpl in *.
+        repeat map_rewrite.
+        assert (balance <> ether);
+          [apply balance_neq_ether|eq_auto].
+        unfold daoFields in *;
+          repeat map_rewrite.
+        assert (balance <> name);
+          [apply balance_neq_name|eq_auto; simpl_crush].
+
+        inversion H10;
+          subst.
+        inversion H17;
+          subst.
+        repeat map_rewrite;
+          simpl in *;
+          unfold χB in *;
+          repeat map_rewrite;
+          simpl_crush.
+        simpl in *;
+          repeat map_rewrite.
+        simpl_crush.
+
+      + inversion H15.
+  Qed.
+
+  Lemma DAO2_sat :
+    DAOModule2 ⊨m DAOSPEC1.
+  Proof.
+    
+  Admitted.
+  
+
+End SimpleDAO.
 
 Module DAOExample.
 
@@ -77,6 +457,7 @@ Module DAOExample.
   (** DAO Definition *)
 
   Definition DAO := classID 1.
+
 
   Definition accountBook := fieldID 3.
 
